<?xml version="1.0" encoding="UTF-8"?>
<?xml-model href="file:/usr/local/share/xml/rdf/rdfxml.rnc" type="application/relax-ng-compact-syntax"?>
<RDF xmlns="http://www.w3.org/1999/02/22-rdf-syntax-ns#"
    xmlns:rdf="http://www.w3.org/1999/02/22-rdf-syntax-ns#"
    xmlns:rdfs="http://www.w3.org/2000/01/rdf-schema#">

    <rdfs:Class rdf:about="Magazine">
        <rdfs:label>Magazine</rdfs:label>
        <rdfs:comment> An abstract serial work comprising
        publications. Equivalent to FRBRoo F18_Serial_Work, cited
        here.</rdfs:comment>
        <rdfs:subClassOf rdf:resource="F18_Serial_Work"/>
    </rdfs:Class>


    <rdfs:Class rdf:about="Number">
        <rdfs:label>Number</rdfs:label>
        <rdfs:comment>One of the periodic publications comprising a
        magazine. Often equivalent to B3_issue, but an issue is the thing
        that's actually published; the number is more conceptual. That is, a
        B2_Number is equivalent to FRBRoo F19_Publication_Work and an issue is
        equivalent to F24_Publication_Expression. An issue can comprise more
        than one number. </rdfs:comment>
        <rdfs:subClassOf rdf:resource="F19_Publication_Work"/>
    </rdfs:Class>


    <rdfs:Class rdf:about="Issue">
        <rdfs:label>Issue</rdfs:label>
        <rdf:comment>A periodic issuance of a magazine. An issue is the
        printed manifestation of one or more conceptual B2_Numbers; it is
        something that is actually published. Equivalent to FRBRoo
        F24_Publication_Expression.</rdf:comment>
        <rdfs:subClassOf rdf:resource="F24_Publication_Expression"/>
    </rdfs:Class>


    <rdfs:Class rdf:about="Copy">
        <rdfs:label>Copy</rdfs:label>
        <rdfs:comment>A physical instance of an issue.</rdfs:comment>
    </rdfs:Class>


    <rdfs:Class rdf:about="Run">
        <rdfs:label>Run</rdfs:label>
        <rdfs:comment>The full, ordered sequence of issues published during
        the lifetime of a magazine.</rdfs:comment>
    </rdfs:Class>


    <rdfs:Class rdf:about="Lifetime">
        <rdfs:label>Lifetime</rdfs:label>
        <rdfs:comment> A timespan starting with the publication date of the
        first issue in the run and ending with the publication date of the
        last issue in the run. </rdfs:comment>
    </rdfs:Class>


    <rdfs:Class rdf:about="Constituent">
      <rdfs:label>Constituent</rdfs:label>
      <rdfs:comment>An identifiable textual or visual element of a
      publication.</rdfs:comment>
    </rdfs:Class>
    

    <rdfs:Class rdf:about="Title">
        <rdfs:label>Title</rdfs:label>
    </rdfs:Class>
</RDF>
